lib/coq/MachineWord.v
@@ -1,0 +1,163 @@
+From Sail Require MachineWordInterface.
+From bbv Require Word.
+Require Arith.
+Require Import ZArith NArith.
+Require Lia.
+Require String.
+Require Strings.Ascii.
+
+Module MachineWord <: MachineWordInterface.MachineWordInterface.
+
+Import List.ListNotations.
+
+Definition dummy {T:Type} (t:T) : T.
+exact t.
+Qed.
+
+Definition cast_word {m n} (x : Word.word m) (eq : m = n) : Word.word n :=
+  DepEqNat.nat_cast _ eq x.
+
+Definition word := Word.word.
+Definition zeros n := @Word.wzero n.
+Definition ones n := @Word.wones n.
+Definition get_bit {n} :=
+  match n with
+  | O => fun (w : Word.word O) i => dummy false
+  | S n => fun (w : Word.word (S n)) i => Word.wlsb (Word.wrshift' w i)
+  end.
+
+Definition set_bit {n} :=
+match n with
+| O => fun (w : Word.word O) i b => w
+| S n => fun (w : Word.word (S n)) i (b : bool) =>
+  let bit : Word.word (S n) := Word.wlshift' (Word.natToWord _ 1) i in
+  let mask : Word.word (S n) := Word.wnot bit in
+  let masked := Word.wand mask w in
+  if b then Word.wor masked bit else masked
+end.
+
+Definition word_to_Z {n} (w : word n) := Word.wordToZ w.
+Definition word_to_N {n} (w : word n) := Word.wordToN w.
+Definition Z_to_word n z := Word.ZToWord n z.
+Definition N_to_word m n := Word.NToWord m n.
+
+Lemma word_to_N_range : forall {n} (w : word n), (word_to_N w < 2 ^ N.of_nat n)%N.
+intros.
+change 2%N with (N.of_nat 2).
+rewrite <- Nat2N.inj_pow.
+rewrite <- NatLib.pow2_N.
+apply Word.wordToN_bound.
+Qed.
+
+Lemma word_to_Z_range : forall {n} (w : word (S n)), (- 2 ^ Z.of_nat n <= word_to_Z w < 2 ^ Z.of_nat n)%Z.
+intros.
+change 2%Z with (Z.of_nat 2).
+rewrite <- Nat2Z.inj_pow.
+apply Word.wordToZ_size'.
+Qed.
+
+Local Fixpoint word_to_bools_aux {n} (w:word n) acc :=
+match w with
+| Word.WO => acc
+| Word.WS b w => word_to_bools_aux w (b::acc)%list
+end.
+
+Definition word_to_bools {n} (w : word n) := word_to_bools_aux w [].
+
+Fixpoint bools_to_word_rev l : word (length l) :=
+match l with
+| [] => Word.WO
+| b::t => Word.WS b (bools_to_word_rev t)
+end%list.
+Definition bools_to_word l : word (length l) :=
+  cast_word (bools_to_word_rev (List.rev l)) (List.rev_length l).
+
+Local Lemma slice_equality {i n m} : i + n <= m -> m = i + (n + (m - n -i)).
+Lia.lia.
+Qed.
+
+Definition slice {m} n (w : word m) (i : nat) : word n :=
+  match Compare_dec.le_lt_dec (i + n) m with
+  | left H =>
+      let w : word (i + (n + (m - n - i))) := cast_word w (slice_equality H) in
+      Word.split1 n _ (Word.split2 i _ w)
+  | right _ => dummy (zeros _)
+  end.
+
+Definition update_slice {m} {n} (w : word m) (i : nat) (v : word n) : word m :=
+  match Compare_dec.le_lt_dec (i + n) m with
+  | left H =>
+    let w : word (i + (n + (m - n - i))) := cast_word w (slice_equality H) in
+    let pre := Word.split1 i _ w in
+    let post := Word.split2 n _ (Word.split2 i _ w) in
+    let w' := Word.combine pre (Word.combine v post) in
+    eq_rect _ _ w' _ (eq_sym (slice_equality H))
+  | right _ => dummy (zeros _)
+  end.
+
+Definition zero_extend {m} n (w : word m) : word n :=
+  match Compare_dec.le_lt_dec m n with
+  | left H =>
+      cast_word (Word.zext w (n - m)) (Arith_prebase.le_plus_minus_r_stt _ _ H)
+  | right _ => dummy (zeros _)
+  end.
+
+Definition sign_extend {m} n (w : word m) : word n :=
+  match Compare_dec.le_lt_dec m n with
+  | left H =>
+      cast_word (Word.sext w (n - m)) (Arith_prebase.le_plus_minus_r_stt _ _ H)
+  | right _ => dummy (zeros _)
+  end.
+
+Definition concat {m n} (w: word m) (v: word n) := Word.combine w v.
+
+Definition and := Word.wand.
+Definition or := Word.wor.
+Definition xor := Word.wxor.
+Definition not := Word.wnot.
+
+Definition add := Word.wplus.
+Definition sub := Word.wminus.
+Definition mul := Word.wmult.
+
+Definition logical_shift_left {n} (w : word n) i := Word.wlshift' w i.
+Definition logical_shift_right {n} (w : word n) i := Word.wrshift' w i.
+Definition arith_shift_right {n} (w : word n) i := Word.wrshifta' w i.
+
+Fixpoint replicate (n : nat) {a} (w : Word.word a) : Word.word (n * a) :=
+match n with
+| O => Word.WO
+| S m => Word.combine w (replicate m w)
+end.
+
+Definition eqb {n} (w v : word n) := Word.weqb w v.
+
+Lemma eqb_true_iff {n} (v w : word n) : eqb v w = true <-> v = w.
+apply Word.weqb_true_iff.
+Qed.
+
+Definition eq_dec {n} (w v : word n) := Word.weq w v.
+
+Fixpoint reverse_endian {n} (bits : word n) : word n :=
+  match n return word n -> word n with
+  | S (S (S (S (S (S (S (S m))))))) => fun bits =>
+    cast_word
+      (Word.combine
+         (reverse_endian (Word.split2 8 m bits))
+         (Word.split1 8 m bits))
+      (PeanoNat.Nat.add_comm _ _)
+  | _ => fun bits => bits
+  end bits.
+
+Import String.
+Import Strings.Ascii.
+
+Local Fixpoint word_to_binary_string_acc {n} (w : Word.word n) (s : string) :=
+  match w with
+  | Word.WO => s
+  | Word.WS b w' => word_to_binary_string_acc w' (String (if b then "1" else "0")%char s)
+  end.
+Definition word_to_binary_string {n} (bv : word n) := String "0" (String "b" (word_to_binary_string_acc bv "")).
+
+
+End MachineWord.
